lean/privacy/notes.lean
@@ -1,0 +1,10 @@
+import privacy.notes.canceled_notes
+import privacy.notes.contiguous
+import privacy.notes.create_note_actions
+import privacy.notes.discoverable_outgoing
+import privacy.notes.discoverable
+import privacy.notes.note_implies
+import privacy.notes.note_owner
+import privacy.notes.notes
+import privacy.notes.open_deposits
+import privacy.notes.scanned_note
